Refactor insert definition
we decouple the focus from the insert definition, and we generalise the
tree stack definitions.

src/Insert_tree_stack.thy
@@ -2,54 +2,70 @@ theory Insert_tree_stack
 imports Tree_stack
 begin
 
-(*begin wfcontext definition*)
-definition subtree_indexes :: "node_t => nat set" where
-"subtree_indexes n == (
-  case n of (l,_) =>  { 0 .. (length l)})"
+(*begin ins focus definition*)
+datatype One_or_two = 
+Inserting_one "Tree"
+| Inserting_two "Tree * key * Tree"
 
-definition is_subnode :: "(node_t * nat) => (node_t * nat) => bool" where
-"is_subnode ni pi == (
-  let (n,_) = ni in
-  let ((ks,rs),i) = pi in
-  Node n = (rs!i))"
-                                        
-fun linked_context :: "(left_bound * (node_t * nat) * right_bound) => context_t => bool" where
-"linked_context ni [] = True" |
-"linked_context (lb,ni,rb) ((plb,pi,prb)#pis) = (
-  is_subnode ni pi & linked_context (plb,pi,prb) pis)"
+type_synonym inserting_two_t =  "Tree * key * Tree"
 
-definition wellformed_context_1 :: "rmbs_t => (left_bound * (node_t * nat) * right_bound) => bool " where
-"wellformed_context_1 rmbs lbnirb == (
-let (lb,((l,cs),i),rb) = lbnirb in
-let node = (Node(l,cs)) in(
-wellformed_tree rmbs node
-& i : (subtree_indexes (l,cs)))
-& check_keys lb (keys node) rb)"
+type_synonym ins_focus_t = One_or_two
+(*end ins focus definition*)
 
-definition get_lower_upper_keys_for_node_t :: "key list => left_bound => nat => right_bound => (key option * key option)" where
-"get_lower_upper_keys_for_node_t ls lb i rb == (
-let l = if (i = 0) then lb else Some(ls ! (i - 1))     in
-let u = if (i = (length ls)) then rb else Some(ls ! i) in
-(l,u)
+(*begin ins_tree_stack definition*)
+type_synonym ins_tree_stack = "ins_focus_t tree_stack"
+(*end ins_tree_stack definition*)
+
+(*begin step ins_tree_stack*)
+definition split_node :: "node_t \<Rightarrow> inserting_two_t" where
+"split_node n == (
+let (l,cs) = n in
+let n0 = min_node_keys in
+let left_ks = take n0 l in
+let (k,right_ks) = (case drop n0 l of (k#ks) \<Rightarrow> (k,ks)) in
+let left_rs = take (1+n0) cs in
+let right_rs = drop (1+n0) cs in
+(Node(left_ks,left_rs),k,Node(right_ks,right_rs))
 )"
 
-fun wellformed_context :: "context_t => bool" where
-"wellformed_context Nil = True" |
-"wellformed_context (x # Nil) = wellformed_context_1 (Rmbs True) x" |
-"wellformed_context (x1 # (x2 # rest)) = (
-let (lb,((ls,_),i),rb) = x2 in
-let (l2,u2) = get_lower_upper_keys_for_node_t ls lb i rb in
-let (l1,_,u1) = x1 in
-wellformed_context_1 (Rmbs False) x1
-& (l1,u1) = (l2,u2)
-& linked_context x1 (x2#rest)
-& wellformed_context (x2#rest)
+definition step_up :: "node_t \<Rightarrow> nat \<Rightarrow> ins_focus_t \<Rightarrow> ins_focus_t" where
+"step_up n i f == (
+let (ks,rs) = n in
+case f of
+Inserting_one t \<Rightarrow> (
+let rs2 = dest_Some(list_replace_1_at_n rs i t) in
+Inserting_one(Node(ks,rs2)))
+| Inserting_two (tl_,k,tr) \<Rightarrow> (
+let ks2 = list_insert_at_n ks i [k] in
+let rs2 = list_replace_at_n rs i [tl_,tr] |> dest_Some in
+case (length ks2 \<le> max_node_keys) of
+True \<Rightarrow> Inserting_one(Node(ks2,rs2))
+| False \<Rightarrow> (
+Inserting_two(split_node(ks2,rs2))
 )
+)
+)"
+
+definition ins_step_tree_stack :: "ins_tree_stack \<Rightarrow> (ins_tree_stack) option" where
+"ins_step_tree_stack ts == (
+let (f,stk) = dest_ts ts in
+case stk of 
+Nil \<Rightarrow> None
+| ((lb,(n,i),rb)#xs) \<Rightarrow> (
+let f2 = step_up n i f in
+Some(Tree_stack((Focus f2),xs))
+)
+
+)
+
 "
-(*end wfcontext definition*)
+
+declare [[code abort: key_lt key_le min_node_keys max_node_keys]]
+export_code ins_step_tree_stack in Scala module_name Insert_tree_stack file "/tmp/Insert_tree_stack.scala"
+(*end step ins_tree_stack*)
 
 (*begin wffocus definition*)
-definition wellformed_focus :: "focus_t => bool => bool" where
+definition wellformed_focus :: "ins_focus_t => bool => bool" where
 "wellformed_focus f stack_empty == (
 case f of
 Inserting_one t => (wellformed_tree (Rmbs stack_empty) t)
@@ -62,7 +78,7 @@ wellformed_tree (Rmbs False) tl_
 (*end wffocus definition*)
 
 (*begin wfts1 definition*)
-definition wellformed_ts_1 :: "tree_stack => bool" where
+definition wellformed_ts_1 :: "ins_tree_stack => bool" where
 "wellformed_ts_1 ts == (
 let (f,stk) = dest_ts ts in
 (case stk of 
@@ -116,7 +132,7 @@ wf
 (*end wfts1 definition*)
 
 (*begin wftreestack definition*)
-definition wellformed_ts :: "tree_stack => bool" where
+definition wellformed_ts :: "ins_tree_stack => bool" where
 "wellformed_ts ts == (
 let (f,stk) = dest_ts ts in
 wellformed_focus f (stk=[])
