src/Tree_stack.thy
@@ -9,8 +9,10 @@ Inserting_one "Tree"
 
 type_synonym inserting_two_t =  "Tree * key * Tree"
 
-type_synonym focus_t = One_or_two
+type_synonym ins_focus_t = One_or_two
 (*end focus definition*)
+
+datatype 'f focus_t = Focus 'f
 
 definition split_node :: "node_t \<Rightarrow> inserting_two_t" where
 "split_node n == (
@@ -23,7 +25,7 @@ let right_rs = drop (1+n0) cs in
 (Node(left_ks,left_rs),k,Node(right_ks,right_rs))
 )"
 
-definition update_focus_at_position :: "node_t \<Rightarrow> nat \<Rightarrow> focus_t \<Rightarrow> focus_t" where
+definition update_focus_at_position :: "node_t \<Rightarrow> nat \<Rightarrow> ins_focus_t \<Rightarrow> ins_focus_t" where
 "update_focus_at_position n i f == (
 let (ks,rs) = n in
 case f of
@@ -50,20 +52,68 @@ type_synonym context_t = "(left_bound * (node_t * nat) * right_bound) list"
 (*end context definition*)
 
 (*begin treestack definition*)
-datatype tree_stack = Tree_stack "focus_t * context_t"
+datatype 'f tree_stack = Tree_stack "'f focus_t * context_t"
 (*end treestack definition*)
 
-definition dest_ts :: "tree_stack \<Rightarrow> focus_t * context_t" where
-"dest_ts ts == (case ts of Tree_stack(f,c) \<Rightarrow> (f,c))"
+(*begin wfcontext definition*)
+definition subtree_indexes :: "node_t => nat set" where
+"subtree_indexes n == (
+  case n of (l,_) =>  { 0 .. (length l)})"
 
-definition step_tree_stack :: "tree_stack \<Rightarrow> tree_stack option" where
+definition is_subnode :: "(node_t * nat) => (node_t * nat) => bool" where
+"is_subnode ni pi == (
+  let (n,_) = ni in
+  let ((ks,rs),i) = pi in
+  Node n = (rs!i))"
+                                        
+fun linked_context :: "(left_bound * (node_t * nat) * right_bound) => context_t => bool" where
+"linked_context ni [] = True" |
+"linked_context (lb,ni,rb) ((plb,pi,prb)#pis) = (
+  is_subnode ni pi & linked_context (plb,pi,prb) pis)"
+
+definition wellformed_context_1 :: "rmbs_t => (left_bound * (node_t * nat) * right_bound) => bool " where
+"wellformed_context_1 rmbs lbnirb == (
+let (lb,((l,cs),i),rb) = lbnirb in
+let node = (Node(l,cs)) in(
+wellformed_tree rmbs node
+& i : (subtree_indexes (l,cs)))
+& check_keys lb (keys node) rb)"
+
+definition get_lower_upper_keys_for_node_t :: "key list => left_bound => nat => right_bound => (key option * key option)" where
+"get_lower_upper_keys_for_node_t ls lb i rb == (
+let l = if (i = 0) then lb else Some(ls ! (i - 1))     in
+let u = if (i = (length ls)) then rb else Some(ls ! i) in
+(l,u)
+)"
+
+fun wellformed_context :: "context_t => bool" where
+"wellformed_context Nil = True" |
+"wellformed_context (x # Nil) = wellformed_context_1 (Rmbs True) x" |
+"wellformed_context (x1 # (x2 # rest)) = (
+let (lb,((ls,_),i),rb) = x2 in
+let (l2,u2) = get_lower_upper_keys_for_node_t ls lb i rb in
+let (l1,_,u1) = x1 in
+wellformed_context_1 (Rmbs False) x1
+& (l1,u1) = (l2,u2)
+& linked_context x1 (x2#rest)
+& wellformed_context (x2#rest)
+)
+"
+(*end wfcontext definition*)
+
+
+definition dest_ts :: "'f tree_stack \<Rightarrow> 'f * context_t" where
+"dest_ts ts == (case ts of Tree_stack((Focus f),c) \<Rightarrow> (f,c))"
+
+
+definition step_tree_stack :: "'f tree_stack \<Rightarrow> ('f tree_stack) option" where
 "step_tree_stack ts == (
 let (f,stk) = dest_ts ts in
 case stk of 
 Nil \<Rightarrow> None
 | ((lb,(n,i),rb)#xs) \<Rightarrow> (
 let f2 = update_focus_at_position n i f in
-Some(Tree_stack(f2,xs))
+Some(Tree_stack((Focus f2),xs))
 )
 
 )
